logrel: use non-atomic invariants and implement the load & store cases

theories/ml_lang/lang.v
@@ -705,10 +705,15 @@ Inductive head_step (p : ml_program) : expr → state → expr → state → Pro
      σ !! Locoff l i = Some v →
      head_step p (StoreN (Val $ LitV $ LitLoc l) (Val $ LitV $ LitInt i) (Val w)) σ
                  (Val $ LitV LitUnit) (<[Locoff l i := w]> σ)
-  (* Silently diverge in case of out-of-bound accesses. We want to distinguish
-     OOB accesses from other failures (which are UB), so that we can prove a
-     type safety result. In a more realistic language we could have a dedicated
-     failure state for OOB, or a mechanism for exceptions/panics... *)
+  (* Silently diverge in case of out-of-bound accesses (or negative alloc size).
+     We want to distinguish OOB accesses from other failures (which are UB),
+     so that we can prove a type safety result. In a more realistic language
+     we could have a dedicated failure state for OOB, or a mechanism for
+     exceptions/panics... *)
+  | AllocNWrongSizeS n v σ :
+    (n < 0)%Z →
+    head_step p (AllocN (Val $ LitV $ LitInt n) (Val v)) σ
+                (AllocN (Val $ LitV $ LitInt n) (Val v)) σ
   | LoadNOobS l i σ :
      σ !! Locoff l i = None →
      head_step p (LoadN (Val $ LitV $ LitLoc l) (Val $ LitV $ LitInt i)) σ
