theories/ml_lang/logrel/typing.v
@@ -13,7 +13,7 @@ Inductive type :=
   | TVar (x : var)
   | TForall (τ : {bind 1 of type})
   | TExist (τ : {bind 1 of type})
-  | Tref (τ : type). (* References are length one. Handling dynamic arrays is difficult *)
+  | TArray (τ : type).
 
 Global Instance Ids_type : Ids type. derive. Defined.
 Global Instance Rename_type : Rename type. derive. Defined.
@@ -42,7 +42,7 @@ Inductive EqType : type → Prop :=
   | EqTUnit : EqType TUnit
   | EqTNat : EqType TNat
   | EqTBool : EqType TBool
-  | EQRef τ : EqType (Tref τ).
+  | EQTArray τ : EqType (TArray τ).
 
 
 Inductive program_type := FunType : list type -> type -> program_type.
@@ -52,58 +52,58 @@ Definition subst_prog_env f (p : program_env) := fmap (subst_prog_type f) p.
 
 Section IndDef.
 
-Reserved Notation "P ; Γ ⊢ₜ e : τ" (at level 74, e, τ at next level).
+Reserved Notation "P ;; Γ ⊢ₜ e : τ" (at level 74, e, τ at next level).
 Unset Elimination Schemes.
 Inductive typed (P : program_env) (Γ : gmap string type) : expr → type → Prop :=
-  | Var_typed x τ : Γ !! x = Some τ → P ; Γ ⊢ₜ Var x : τ 
-  | Unit_typed : P ; Γ ⊢ₜ  #LitUnit : TUnit
-  | Nat_typed (n:Z) : P ; Γ ⊢ₜ # n : TNat
-  | Bool_typed (b:bool) : P ; Γ ⊢ₜ # b : TBool
+  | Var_typed x τ : Γ !! x = Some τ → P ;; Γ ⊢ₜ Var x : τ
+  | Unit_typed : P ;; Γ ⊢ₜ  #LitUnit : TUnit
+  | Nat_typed (n:Z) : P ;; Γ ⊢ₜ # n : TNat
+  | Bool_typed (b:bool) : P ;; Γ ⊢ₜ # b : TBool
   | BinOp_typed_nat_nat op e1 e2 :
      binop_arithmetic op = true → 
-     P ; Γ ⊢ₜ e1 : TNat → P ; Γ ⊢ₜ e2 : TNat → P ; Γ ⊢ₜ BinOp op e1 e2 : TNat
+     P ;; Γ ⊢ₜ e1 : TNat → P ;; Γ ⊢ₜ e2 : TNat → P ;; Γ ⊢ₜ BinOp op e1 e2 : TNat
   | BinOp_typed_nat_bool op e1 e2 :
      binop_arithmetic_to_bool op = true → 
-     P ; Γ ⊢ₜ e1 : TNat → P ; Γ ⊢ₜ e2 : TNat → P ; Γ ⊢ₜ BinOp op e1 e2 : TBool
+     P ;; Γ ⊢ₜ e1 : TNat → P ;; Γ ⊢ₜ e2 : TNat → P ;; Γ ⊢ₜ BinOp op e1 e2 : TBool
   | BinOp_typed_bool op e1 e2 :
      binop_boolish op = true → 
-     P ; Γ ⊢ₜ e1 : TBool → P ; Γ ⊢ₜ e2 : TBool → P ; Γ ⊢ₜ BinOp op e1 e2 : TBool
+     P ;; Γ ⊢ₜ e1 : TBool → P ;; Γ ⊢ₜ e2 : TBool → P ;; Γ ⊢ₜ BinOp op e1 e2 : TBool
   | BinOp_typed_eq T e1 e2 :
      EqType T → 
-     P ; Γ ⊢ₜ e1 : T → P ; Γ ⊢ₜ e2 : T → P ; Γ ⊢ₜ BinOp EqOp e1 e2 : TBool
-  | Pair_typed e1 e2 τ1 τ2 : P ; Γ ⊢ₜ e1 : τ1 → P ; Γ ⊢ₜ e2 : τ2 → P ; Γ ⊢ₜ Pair e1 e2 : TProd τ1 τ2
-  | Fst_typed e τ1 τ2 : P ; Γ ⊢ₜ e : TProd τ1 τ2 → P ; Γ ⊢ₜ Fst e : τ1
-  | Snd_typed e τ1 τ2 : P ; Γ ⊢ₜ e : TProd τ1 τ2 → P ; Γ ⊢ₜ Snd e : τ2
-  | InjL_typed e τ1 τ2 : P ; Γ ⊢ₜ e : τ1 → P ; Γ ⊢ₜ InjL e : TSum τ1 τ2
-  | InjR_typed e τ1 τ2 : P ; Γ ⊢ₜ e : τ2 → P ; Γ ⊢ₜ InjR e : TSum τ1 τ2
+     P ;; Γ ⊢ₜ e1 : T → P ;; Γ ⊢ₜ e2 : T → P ;; Γ ⊢ₜ BinOp EqOp e1 e2 : TBool
+  | Pair_typed e1 e2 τ1 τ2 : P ;; Γ ⊢ₜ e1 : τ1 → P ;; Γ ⊢ₜ e2 : τ2 → P ;; Γ ⊢ₜ Pair e1 e2 : TProd τ1 τ2
+  | Fst_typed e τ1 τ2 : P ;; Γ ⊢ₜ e : TProd τ1 τ2 → P ;; Γ ⊢ₜ Fst e : τ1
+  | Snd_typed e τ1 τ2 : P ;; Γ ⊢ₜ e : TProd τ1 τ2 → P ;; Γ ⊢ₜ Snd e : τ2
+  | InjL_typed e τ1 τ2 : P ;; Γ ⊢ₜ e : τ1 → P ;; Γ ⊢ₜ InjL e : TSum τ1 τ2
+  | InjR_typed e τ1 τ2 : P ;; Γ ⊢ₜ e : τ2 → P ;; Γ ⊢ₜ InjR e : TSum τ1 τ2
   | Case_typed e0 e1 e2 τ1 τ2 τ3 :
-     P ; Γ ⊢ₜ e0 : TSum τ1 τ2 → P ; Γ ⊢ₜ e1 : (TArrow τ1 τ3) → P ; Γ ⊢ₜ e2 : (TArrow τ2 τ3) →
-     P ; Γ ⊢ₜ Case e0 e1 e2 : τ3
+     P ;; Γ ⊢ₜ e0 : TSum τ1 τ2 → P ;; Γ ⊢ₜ e1 : (TArrow τ1 τ3) → P ;; Γ ⊢ₜ e2 : (TArrow τ2 τ3) →
+     P ;; Γ ⊢ₜ Case e0 e1 e2 : τ3
   | If_typed e0 e1 e2 τ :
-     P ; Γ ⊢ₜ e0 : TBool → P ; Γ ⊢ₜ e1 : τ → P ; Γ ⊢ₜ e2 : τ → P ; Γ ⊢ₜ If e0 e1 e2 : τ
+     P ;; Γ ⊢ₜ e0 : TBool → P ;; Γ ⊢ₜ e1 : τ → P ;; Γ ⊢ₜ e2 : τ → P ;; Γ ⊢ₜ If e0 e1 e2 : τ
   | Rec_typed f x e τ1 τ2 :
-     P ; (binder_insert f (TArrow τ1 τ2) (binder_insert x τ1 Γ)) ⊢ₜ e : τ2 → P ; Γ ⊢ₜ Rec f x e : TArrow τ1 τ2
+     P ;; (binder_insert f (TArrow τ1 τ2) (binder_insert x τ1 Γ)) ⊢ₜ e : τ2 → P ;; Γ ⊢ₜ Rec f x e : TArrow τ1 τ2
   | App_typed e1 e2 τ1 τ2 :
-     P ; Γ ⊢ₜ e1 : TArrow τ1 τ2 → P ; Γ ⊢ₜ e2 : τ1 → P ; Γ ⊢ₜ App e1 e2 : τ2
+     P ;; Γ ⊢ₜ e1 : TArrow τ1 τ2 → P ;; Γ ⊢ₜ e2 : τ1 → P ;; Γ ⊢ₜ App e1 e2 : τ2
   | TLam_typed e τ :
-     subst_prog_env (ren (+1)) P ; subst (ren (+1)) <$> Γ ⊢ₜ e : τ → P ; Γ ⊢ₜ TLam e : TForall τ
-  | TApp_typed e τ τ' : P ; Γ ⊢ₜ e : TForall τ → P ; Γ ⊢ₜ TApp e : τ.[τ'/]
+     subst_prog_env (ren (+1)) P ;; subst (ren (+1)) <$> Γ ⊢ₜ e : τ → P ;; Γ ⊢ₜ TLam e : TForall τ
+  | TApp_typed e τ τ' : P ;; Γ ⊢ₜ e : TForall τ → P ;; Γ ⊢ₜ TApp e : τ.[τ'/]
   | Pack_typed e τ τ' :
-     P ; Γ ⊢ₜ e : τ.[τ'/] → P ; Γ ⊢ₜ Pack e : TExist τ
+     P ;; Γ ⊢ₜ e : τ.[τ'/] → P ;; Γ ⊢ₜ Pack e : TExist τ
   | UnpackIn_typed x e1 e2 τ τ' :
-     P ; Γ ⊢ₜ e1 : TExist τ →
-     subst_prog_env (ren (+1)) P ; binder_insert x τ (subst (ren (+1)) <$> Γ) ⊢ₜ e2 : τ'.[ren (+1)] →
-     P ; Γ ⊢ₜ UnpackIn x e1 e2 : τ'
-  | TRoll e τ : P ; Γ ⊢ₜ e : τ.[TRec τ/] → P ; Γ ⊢ₜ Roll e : TRec τ
-  | TUnroll e τ : P ; Γ ⊢ₜ e : TRec τ → P ; Γ ⊢ₜ Unroll e : τ.[TRec τ/] 
-  | TAlloc e τ : P ; Γ ⊢ₜ e : τ → P ; Γ ⊢ₜ ref e : Tref τ 
-  | TLoad e τ : P ; Γ ⊢ₜ e : Tref τ → P ; Γ ⊢ₜ Load e #0 : τ 
-  | TStore e e' τ : P ; Γ ⊢ₜ e : Tref τ → P ; Γ ⊢ₜ e' : τ → P ; Γ ⊢ₜ Store e (#0) e' : TUnit 
+     P ;; Γ ⊢ₜ e1 : TExist τ →
+     subst_prog_env (ren (+1)) P ;; binder_insert x τ (subst (ren (+1)) <$> Γ) ⊢ₜ e2 : τ'.[ren (+1)] →
+     P ;; Γ ⊢ₜ UnpackIn x e1 e2 : τ'
+  | TRoll e τ : P ;; Γ ⊢ₜ e : τ.[TRec τ/] → P ;; Γ ⊢ₜ Roll e : TRec τ
+  | TUnroll e τ : P ;; Γ ⊢ₜ e : TRec τ → P ;; Γ ⊢ₜ Unroll e : τ.[TRec τ/]
+  | TAllocN e1 e2 τ : P ;; Γ ⊢ₜ e1 : TNat → P ;; Γ ⊢ₜ e2 : τ → P ;; Γ ⊢ₜ AllocN e1 e2 : TArray τ
+  | TLoadN e1 e2 τ : P ;; Γ ⊢ₜ e1 : TArray τ → P ;; Γ ⊢ₜ e2 : TNat → P ;; Γ ⊢ₜ LoadN e1 e2 : τ
+  | TStoreN e1 e2 e3 τ : P ;; Γ ⊢ₜ e1 : TArray τ → P ;; Γ ⊢ₜ e2 : TNat → P ;; Γ ⊢ₜ e3 : τ → P ;; Γ ⊢ₜ StoreN e1 e2 e3 : TUnit
   | TExtern s el tl tr :
       P !! s = Some (FunType tl tr) →
       Forall2 (typed P Γ) el tl →
-      P ; Γ ⊢ₜ (Extern s el) : tr
-where "P ; Γ ⊢ₜ e : τ" := (typed P Γ e τ).
+      P ;; Γ ⊢ₜ (Extern s el) : tr
+where "P ;; Γ ⊢ₜ e : τ" := (typed P Γ e τ).
 
 (* Forall2 (typed Γ) requires special care *)
 Lemma typed_ind (P : program_env → gmap string type → expr → type → Prop) : 
@@ -111,30 +111,30 @@ Lemma typed_ind (P : program_env → gmap string type → expr → type → Prop
   → (∀ (P0 : program_env) (Γ : gmap string type), P P0 Γ #() TUnit)
   → (∀ (P0 : program_env) (Γ : gmap string type) (n : Z), P P0 Γ #n TNat)
   → (∀ (P0 : program_env) (Γ : gmap string type) (b : bool), P P0 Γ #b TBool)
-  → (∀ (P0 : program_env) (Γ : gmap string type) (op : bin_op) (e1 e2 : expr), binop_arithmetic op = true → P0; Γ ⊢ₜ e1 : TNat → P P0 Γ e1 TNat → P0; Γ ⊢ₜ e2 : TNat → P P0 Γ e2 TNat → P P0 Γ (BinOp op e1 e2) TNat)
-  → (∀ (P0 : program_env) (Γ : gmap string type) (op : bin_op) (e1 e2 : expr), binop_arithmetic_to_bool op = true → P0; Γ ⊢ₜ e1 : TNat → P P0 Γ e1 TNat → P0; Γ ⊢ₜ e2 : TNat → P P0 Γ e2 TNat → P P0 Γ (BinOp op e1 e2) TBool)
-  → (∀ (P0 : program_env) (Γ : gmap string type) (op : bin_op) (e1 e2 : expr), binop_boolish op = true → P0; Γ ⊢ₜ e1 : TBool → P P0 Γ e1 TBool → P0; Γ ⊢ₜ e2 : TBool → P P0 Γ e2 TBool → P P0 Γ (BinOp op e1 e2) TBool)
-  → (∀ (P0 : program_env) (Γ : gmap string type) (T : type) (e1 e2 : expr), EqType T → P0; Γ ⊢ₜ e1 : T → P P0 Γ e1 T → P0; Γ ⊢ₜ e2 : T → P P0 Γ e2 T → P P0 Γ (BinOp EqOp e1 e2) TBool)
-  → (∀ (P0 : program_env) (Γ : gmap string type) (e1 e2 : expr) (τ1 τ2 : type), P0; Γ ⊢ₜ e1 : τ1 → P P0 Γ e1 τ1 → P0; Γ ⊢ₜ e2 : τ2 → P P0 Γ e2 τ2 → P P0 Γ (e1, e2)%MLE (TProd τ1 τ2))
-  → (∀ (P0 : program_env) (Γ : gmap string type) (e : expr) (τ1 τ2 : type), P0; Γ ⊢ₜ e : TProd τ1 τ2 → P P0 Γ e (TProd τ1 τ2) → P P0 Γ (Fst e) τ1)
-  → (∀ (P0 : program_env) (Γ : gmap string type) (e : expr) (τ1 τ2 : type), P0; Γ ⊢ₜ e : TProd τ1 τ2 → P P0 Γ e (TProd τ1 τ2) → P P0 Γ (Snd e) τ2)
-  → (∀ (P0 : program_env) (Γ : gmap string type) (e : expr) (τ1 τ2 : type), P0; Γ ⊢ₜ e : τ1 → P P0 Γ e τ1 → P P0 Γ (InjL e) (TSum τ1 τ2))
-  → (∀ (P0 : program_env) (Γ : gmap string type) (e : expr) (τ1 τ2 : type), P0; Γ ⊢ₜ e : τ2 → P P0 Γ e τ2 → P P0 Γ (InjR e) (TSum τ1 τ2))
-  → (∀ (P0 : program_env) (Γ : gmap string type) (e0 e1 e2 : expr) (τ1 τ2 τ3 : type), P0; Γ ⊢ₜ e0 : TSum τ1 τ2 → P P0 Γ e0 (TSum τ1 τ2) → P0; Γ ⊢ₜ e1 : TArrow τ1 τ3 → P P0 Γ e1 (TArrow τ1 τ3) → P0; Γ ⊢ₜ e2 : TArrow τ2 τ3 → P P0 Γ e2 (TArrow τ2 τ3) → P P0 Γ (Case e0 e1 e2) τ3)
-  → (∀ (P0 : program_env) (Γ : gmap string type) (e0 e1 e2 : expr) (τ : type), P0; Γ ⊢ₜ e0 : TBool → P P0 Γ e0 TBool → P0; Γ ⊢ₜ e1 : τ → P P0 Γ e1 τ → P0; Γ ⊢ₜ e2 : τ → P P0 Γ e2 τ → P P0 Γ (if: e0 then e1 else e2)%MLE τ)
-  → (∀ (P0 : program_env) (Γ : gmap string type) (f14 x : binder) (e : expr) (τ1 τ2 : type), P0; binder_insert f14 (TArrow τ1 τ2) (binder_insert x τ1 Γ) ⊢ₜ e : τ2 → P P0 (binder_insert f14 (TArrow τ1 τ2) (binder_insert x τ1 Γ)) e τ2 → P P0 Γ (rec: f14 x := e)%MLE (TArrow τ1 τ2))
-  → (∀ (P0 : program_env) (Γ : gmap string type) (e1 e2 : expr) (τ1 τ2 : type), P0; Γ ⊢ₜ e1 : TArrow τ1 τ2 → P P0 Γ e1 (TArrow τ1 τ2) → P0; Γ ⊢ₜ e2 : τ1 → P P0 Γ e2 τ1 → P P0 Γ (e1 e2) τ2)
-  → (∀ (P0 : program_env) (Γ : gmap string type) (e : expr) (τ : type), subst_prog_env (ren (+1)) P0; subst (ren (+1)) <$> Γ ⊢ₜ e : τ → P (subst_prog_env (ren (+1)) P0) (subst (ren (+1)) <$> Γ) e τ → P P0 Γ (Λ: <>, e)%MLE (TForall τ))
-  → (∀ (P0 : program_env) (Γ : gmap string type) (e : expr) (τ τ' : {bind type}), P0; Γ ⊢ₜ e : TForall τ → P P0 Γ e (TForall τ) → P P0 Γ (TApp e) τ.[τ'/])
-  → (∀ (P0 : program_env) (Γ : gmap string type) (e : expr) (τ τ' : type), P0; Γ ⊢ₜ e : τ.[τ'/] → P P0 Γ e τ.[τ'/] → P P0 Γ (pack:e)%MLE (TExist τ))
-  → (∀ (P0 : program_env) (Γ : gmap string type) (x : binder) (e1 e2 : expr) (τ : {bind type}) (τ' : type), P0; Γ ⊢ₜ e1 : TExist τ → P P0 Γ e1 (TExist τ) → subst_prog_env (ren (+1)) P0; binder_insert x τ (subst (ren (+1)) <$> Γ) ⊢ₜ e2 : τ'.[ren (+1)] → P (subst_prog_env (ren (+1)) P0) (binder_insert x τ (subst (ren (+1)) <$> Γ)) e2 τ'.[ren (+1)] → P P0 Γ (unpack: x := e2 in e1)%MLE τ')
-  → (∀ (P0 : program_env) (Γ : gmap string type) (e : expr) (τ : {bind type}), P0; Γ ⊢ₜ e : τ.[TRec τ/] → P P0 Γ e τ.[TRec τ/] → P P0 Γ (roll:e)%MLE (TRec τ))
-  → (∀ (P0 : program_env) (Γ : gmap string type) (e : expr) (τ : {bind type}), P0; Γ ⊢ₜ e : TRec τ → P P0 Γ e (TRec τ) → P P0 Γ (unroll:e)%MLE τ.[TRec τ/])
-  → (∀ (P0 : program_env) (Γ : gmap string type) (e : expr) (τ : type), P0; Γ ⊢ₜ e : τ → P P0 Γ e τ → P P0 Γ (ref e)%MLE (Tref τ))
-  → (∀ (P0 : program_env) (Γ : gmap string type) (e : expr) (τ : type), P0; Γ ⊢ₜ e : Tref τ → P P0 Γ e (Tref τ) → P P0 Γ ((! e)%MLE #0) τ)
-  → (∀ (P0 : program_env) (Γ : gmap string type) (e e' : expr) (τ : type), P0; Γ ⊢ₜ e : Tref τ → P P0 Γ e (Tref τ) → P0; Γ ⊢ₜ e' : τ → P P0 Γ e' τ → P P0 Γ ((e <- #0)%MLE e') TUnit)
+  → (∀ (P0 : program_env) (Γ : gmap string type) (op : bin_op) (e1 e2 : expr), binop_arithmetic op = true → P0;; Γ ⊢ₜ e1 : TNat → P P0 Γ e1 TNat → P0;; Γ ⊢ₜ e2 : TNat → P P0 Γ e2 TNat → P P0 Γ (BinOp op e1 e2) TNat)
+  → (∀ (P0 : program_env) (Γ : gmap string type) (op : bin_op) (e1 e2 : expr), binop_arithmetic_to_bool op = true → P0;; Γ ⊢ₜ e1 : TNat → P P0 Γ e1 TNat → P0;; Γ ⊢ₜ e2 : TNat → P P0 Γ e2 TNat → P P0 Γ (BinOp op e1 e2) TBool)
+  → (∀ (P0 : program_env) (Γ : gmap string type) (op : bin_op) (e1 e2 : expr), binop_boolish op = true → P0;; Γ ⊢ₜ e1 : TBool → P P0 Γ e1 TBool → P0;; Γ ⊢ₜ e2 : TBool → P P0 Γ e2 TBool → P P0 Γ (BinOp op e1 e2) TBool)
+  → (∀ (P0 : program_env) (Γ : gmap string type) (T : type) (e1 e2 : expr), EqType T → P0;; Γ ⊢ₜ e1 : T → P P0 Γ e1 T → P0;; Γ ⊢ₜ e2 : T → P P0 Γ e2 T → P P0 Γ (BinOp EqOp e1 e2) TBool)
+  → (∀ (P0 : program_env) (Γ : gmap string type) (e1 e2 : expr) (τ1 τ2 : type), P0;; Γ ⊢ₜ e1 : τ1 → P P0 Γ e1 τ1 → P0;; Γ ⊢ₜ e2 : τ2 → P P0 Γ e2 τ2 → P P0 Γ (e1, e2)%MLE (TProd τ1 τ2))
+  → (∀ (P0 : program_env) (Γ : gmap string type) (e : expr) (τ1 τ2 : type), P0;; Γ ⊢ₜ e : TProd τ1 τ2 → P P0 Γ e (TProd τ1 τ2) → P P0 Γ (Fst e) τ1)
+  → (∀ (P0 : program_env) (Γ : gmap string type) (e : expr) (τ1 τ2 : type), P0;; Γ ⊢ₜ e : TProd τ1 τ2 → P P0 Γ e (TProd τ1 τ2) → P P0 Γ (Snd e) τ2)
+  → (∀ (P0 : program_env) (Γ : gmap string type) (e : expr) (τ1 τ2 : type), P0;; Γ ⊢ₜ e : τ1 → P P0 Γ e τ1 → P P0 Γ (InjL e) (TSum τ1 τ2))
+  → (∀ (P0 : program_env) (Γ : gmap string type) (e : expr) (τ1 τ2 : type), P0;; Γ ⊢ₜ e : τ2 → P P0 Γ e τ2 → P P0 Γ (InjR e) (TSum τ1 τ2))
+  → (∀ (P0 : program_env) (Γ : gmap string type) (e0 e1 e2 : expr) (τ1 τ2 τ3 : type), P0;; Γ ⊢ₜ e0 : TSum τ1 τ2 → P P0 Γ e0 (TSum τ1 τ2) → P0;; Γ ⊢ₜ e1 : TArrow τ1 τ3 → P P0 Γ e1 (TArrow τ1 τ3) → P0;; Γ ⊢ₜ e2 : TArrow τ2 τ3 → P P0 Γ e2 (TArrow τ2 τ3) → P P0 Γ (Case e0 e1 e2) τ3)
+  → (∀ (P0 : program_env) (Γ : gmap string type) (e0 e1 e2 : expr) (τ : type), P0;; Γ ⊢ₜ e0 : TBool → P P0 Γ e0 TBool → P0;; Γ ⊢ₜ e1 : τ → P P0 Γ e1 τ → P0;; Γ ⊢ₜ e2 : τ → P P0 Γ e2 τ → P P0 Γ (if: e0 then e1 else e2)%MLE τ)
+  → (∀ (P0 : program_env) (Γ : gmap string type) (f14 x : binder) (e : expr) (τ1 τ2 : type), P0;; binder_insert f14 (TArrow τ1 τ2) (binder_insert x τ1 Γ) ⊢ₜ e : τ2 → P P0 (binder_insert f14 (TArrow τ1 τ2) (binder_insert x τ1 Γ)) e τ2 → P P0 Γ (rec: f14 x := e)%MLE (TArrow τ1 τ2))
+  → (∀ (P0 : program_env) (Γ : gmap string type) (e1 e2 : expr) (τ1 τ2 : type), P0;; Γ ⊢ₜ e1 : TArrow τ1 τ2 → P P0 Γ e1 (TArrow τ1 τ2) → P0;; Γ ⊢ₜ e2 : τ1 → P P0 Γ e2 τ1 → P P0 Γ (e1 e2) τ2)
+  → (∀ (P0 : program_env) (Γ : gmap string type) (e : expr) (τ : type), subst_prog_env (ren (+1)) P0;; subst (ren (+1)) <$> Γ ⊢ₜ e : τ → P (subst_prog_env (ren (+1)) P0) (subst (ren (+1)) <$> Γ) e τ → P P0 Γ (Λ: <>, e)%MLE (TForall τ))
+  → (∀ (P0 : program_env) (Γ : gmap string type) (e : expr) (τ τ' : {bind type}), P0;; Γ ⊢ₜ e : TForall τ → P P0 Γ e (TForall τ) → P P0 Γ (TApp e) τ.[τ'/])
+  → (∀ (P0 : program_env) (Γ : gmap string type) (e : expr) (τ τ' : type), P0;; Γ ⊢ₜ e : τ.[τ'/] → P P0 Γ e τ.[τ'/] → P P0 Γ (pack:e)%MLE (TExist τ))
+  → (∀ (P0 : program_env) (Γ : gmap string type) (x : binder) (e1 e2 : expr) (τ : {bind type}) (τ' : type), P0;; Γ ⊢ₜ e1 : TExist τ → P P0 Γ e1 (TExist τ) → subst_prog_env (ren (+1)) P0;; binder_insert x τ (subst (ren (+1)) <$> Γ) ⊢ₜ e2 : τ'.[ren (+1)] → P (subst_prog_env (ren (+1)) P0) (binder_insert x τ (subst (ren (+1)) <$> Γ)) e2 τ'.[ren (+1)] → P P0 Γ (unpack: x := e2 in e1)%MLE τ')
+  → (∀ (P0 : program_env) (Γ : gmap string type) (e : expr) (τ : {bind type}), P0;; Γ ⊢ₜ e : τ.[TRec τ/] → P P0 Γ e τ.[TRec τ/] → P P0 Γ (roll:e)%MLE (TRec τ))
+  → (∀ (P0 : program_env) (Γ : gmap string type) (e : expr) (τ : {bind type}), P0;; Γ ⊢ₜ e : TRec τ → P P0 Γ e (TRec τ) → P P0 Γ (unroll:e)%MLE τ.[TRec τ/])
+  → (∀ (P0 : program_env) (Γ : gmap string type) (e1 e2 : expr) (τ : type), P0;; Γ ⊢ₜ e1 : TNat → P P0 Γ e1 TNat → P0;; Γ ⊢ₜ e2 : τ → P P0 Γ e2 τ → P P0 Γ (AllocN e1 e2) (TArray τ))
+  → (∀ (P0 : program_env) (Γ : gmap string type) (e1 e2 : expr) (τ : type), P0;; Γ ⊢ₜ e1 : TArray τ → P P0 Γ e1 (TArray τ) → P0;; Γ ⊢ₜ e2 : TNat → P P0 Γ e2 TNat → P P0 Γ (LoadN e1 e2) τ)
+  → (∀ (P0 : program_env) (Γ : gmap string type) (e1 e2 e3 : expr) (τ : type), P0;; Γ ⊢ₜ e1 : TArray τ → P P0 Γ e1 (TArray τ) → P0;; Γ ⊢ₜ e2 : TNat → P P0 Γ e2 TNat → P0;; Γ ⊢ₜ e3 : τ → P P0 Γ e3 τ → P P0 Γ (StoreN e1 e2 e3) TUnit)
   → (∀ (P0 : program_env) (Γ : gmap string type) (s : string) (el : list expr) (tl : list type) (tr : type), P0 !! s = Some (FunType tl tr) → Forall2 (typed P0 Γ) el tl → Forall2 (P P0 Γ) el tl → P P0 Γ (Extern s el) tr) 
-  →  ∀ (P0 : program_env) (Γ : gmap string type) (e : expr) (t : type), P0; Γ ⊢ₜ e : t → P P0 Γ e t.
+  →  ∀ (P0 : program_env) (Γ : gmap string type) (e : expr) (t : type), P0;; Γ ⊢ₜ e : t → P P0 Γ e t.
 Proof.
   do 27 intros ?.
   fix IH 5. intros ????; destruct 1; eauto 5.
@@ -154,7 +154,7 @@ Proof.
   intros H. cbn. rewrite H. done.
 Qed.
 
-Lemma typed_closed P Γ τ e : P ; Γ ⊢ₜ e : τ → is_closed_expr (dom Γ) e.
+Lemma typed_closed P Γ τ e : P ;; Γ ⊢ₜ e : τ → is_closed_expr (dom Γ) e.
 Proof.
   intros H; induction H using typed_ind; cbn; eauto.
   - by eapply bool_decide_pack, elem_of_dom_2.
@@ -162,7 +162,6 @@ Proof.
     destruct x, f14; cbn in *; try apply IHtyped.
   - by erewrite dom_fmap_L in IHtyped.
   - rewrite !dom_binder_insert !dom_fmap_L in IHtyped2. eauto.
-  - eauto 10.
   - eapply forallb_True, Forall2_Forall_l. 1:done.
     eapply Forall_true. done.
 Qed.
@@ -170,4 +169,4 @@ Set Elimination Schemes.
 End IndDef.
 
 
-Notation "P ; Γ ⊢ₜ e : τ" := (typed P Γ e τ) (at level 74, e, τ at next level).
+Notation "P ;; Γ ⊢ₜ e : τ" := (typed P Γ e τ) (at level 74, e, τ at next level).
