theories/ml_lang/logrel/fundamental.v
@@ -1,17 +1,17 @@
-From iris.base_logic Require Import invariants.
+From iris.base_logic.lib Require Import na_invariants.
 From melocoton.language Require Import lifting.
 From iris.proofmode Require Import proofmode.
 From melocoton.ml_lang.logrel Require Export logrel typing.
 From Autosubst Require Export Autosubst.
 From iris.prelude Require Import options.
 
-Definition log_typed `{!heapGS_ML Σ, !invGS_gen hlc Σ} {p:prog_environ ML_lang Σ} (P : program_env) (Γ : gmap string type) (e : expr) (τ : type) : iProp Σ :=
+Definition log_typed `{!heapGS_ML Σ, !invGS_gen hlc Σ, !logrel_na_invs Σ} {p:prog_environ ML_lang Σ} (P : program_env) (Γ : gmap string type) (e : expr) (τ : type) : iProp Σ :=
   □ ∀ Δ vs, ⟦ Γ ⟧* p Δ vs -∗ ⟦ P ⟧ₚ* p Δ -∗ ⟦ τ ⟧ₑ p Δ (env_subst vs e).
-Notation "P ; Γ ⊨ e : τ" := (log_typed P Γ e τ) (at level 74, Γ, e, τ at next level).
+Notation "P  ;;  Γ  ⊨  e  :  τ" := (log_typed P Γ e τ) (at level 74, Γ, e, τ at next level).
 
 
 Section typed_interp.
-  Context `{!heapGS_ML Σ, !invGS_gen hlc Σ}.
+  Context `{!heapGS_ML Σ, !invGS_gen hlc Σ, !logrel_na_invs Σ}.
   Context {p:prog_environ ML_lang Σ}.
   Notation D := (persistent_predO val (iPropI Σ)).
 
@@ -19,172 +19,183 @@ Section typed_interp.
   Notation "⟦ τ ⟧ x " := (interp p τ x) (at level 10).
   Notation "⟦ τ ⟧ₑ x" := (interp_expr p τ x) (at level 10).
   Notation "⟦ Γ ⟧* x" := (interp_env p Γ x) (at level 10).
-  Notation "P ; Γ ⊨ e : τ" := (log_typed (p:=p) P Γ e τ) (at level 74, Γ, e, τ at next level).
+  Notation "P  ;;  Γ  ⊨  e  :  τ" := (log_typed (p:=p) P Γ e τ) (at level 74, Γ, e, τ at next level).
 
   Lemma interp_expr_bind K e Δ τ τ' :
     ⟦ τ ⟧ₑ Δ e -∗ (∀ v, ⟦ τ ⟧ Δ v -∗ ⟦ τ' ⟧ₑ Δ (fill K (of_val v))) -∗ ⟦ τ' ⟧ₑ Δ (fill K e).
-  Proof. iIntros; iApply wp_bind; iApply (wp_wand with "[$]"); done. Qed.
+  Proof.
+    iIntros "He Hcont Htok". iApply wp_bind.
+    iApply (wp_wand with "[He Htok]").
+    { iSpecialize ("He" with "Htok"). done. }
+    cbn. iIntros (v) "[Hv Htok]".
+    iSpecialize ("Hcont" with "Hv Htok"). done.
+  Qed.
 
   Lemma sem_typed_var P Γ x τ :
-    Γ !! x = Some τ → ⊢ P ; Γ ⊨ Var x : τ.
+    Γ !! x = Some τ → ⊢ P ;; Γ ⊨ Var x : τ.
   Proof.
     iIntros (? Δ vs) "!# #HΓ #HP"; simpl.
     iDestruct (interp_env_Some_l with "HΓ") as (v) "[% ?]"; first done.
-    rewrite H0.
-    iApply wp_value; done.
+    rewrite H0. iIntros "Htok". iApply wp_value; eauto.
   Qed.
 
-  Lemma sem_typed_unit P Γ : ⊢ P ; Γ ⊨ # LitUnit : TUnit.
-  Proof. iIntros (Δ vs) "!# #HΓ #HP". iApply wp_value; done. Qed.
+  Lemma sem_typed_unit P Γ : ⊢ P ;; Γ ⊨ # LitUnit : TUnit.
+  Proof. iIntros (Δ vs) "!# #HΓ #HP Htok". iApply wp_value; eauto. Qed.
 
-  Lemma sem_typed_nat P Γ (n:Z) : ⊢ P ; Γ ⊨ # n : TNat.
-  Proof. iIntros (Δ vs) "!# #HΓ #HP /=". iApply wp_value; eauto. Qed.
+  Lemma sem_typed_nat P Γ (n:Z) : ⊢ P ;; Γ ⊨ # n : TNat.
+  Proof. iIntros (Δ vs) "!# #HΓ #HP /= Htok". iApply wp_value; eauto. Qed.
 
-  Lemma sem_typed_bool P Γ (b:bool) : ⊢ P ; Γ ⊨ # b : TBool.
-  Proof. iIntros (Δ vs) "!# #HΓ #HP /=". iApply wp_value; eauto. Qed.
+  Lemma sem_typed_bool P Γ (b:bool) : ⊢ P ;; Γ ⊨ # b : TBool.
+  Proof. iIntros (Δ vs) "!# #HΓ #HP /= Htok". iApply wp_value; eauto. Qed.
 
   Lemma sem_typed_nat_binop P Γ op e1 e2 :
     binop_arithmetic op = true →
-    P ; Γ ⊨ e1 : TNat -∗ P ; Γ ⊨ e2 : TNat -∗ P ; Γ ⊨ BinOp op e1 e2 : TNat.
+    P ;; Γ ⊨ e1 : TNat -∗ P ;; Γ ⊨ e2 : TNat -∗ P ;; Γ ⊨ BinOp op e1 e2 : TNat.
   Proof.
     iIntros (Hop) "#IH1 #IH2". iIntros (Δ vs) "!# #HΓ #HP /=".
-    iApply (interp_expr_bind [BinOpRCtx _ _]); first by iApply "IH2".
+    iApply (interp_expr_bind [BinOpRCtx _ _]); first (by iApply "IH2"; last done).
     iIntros (v) "#Hv /=".
-    iApply (interp_expr_bind [BinOpLCtx _ _]); first by iApply "IH1".
-    iIntros (w) "#Hw/=".
+    iApply (interp_expr_bind [BinOpLCtx _ _]); first (by iApply "IH1"; last done).
+    iIntros (w) "#Hw/= Htok".
     iDestruct "Hv" as (n) "%"; iDestruct "Hw" as (n') "%"; simplify_eq/=.
     assert (exists (nr:Z), bin_op_eval op (#n') (#n) = Some (#nr)) as [nr Hnr].
     1: { destruct op. 1-10: by eexists. all: cbn in Hop; done. }
     iApply wp_pure_step_later; [done|]; iIntros "!>". iApply wp_value; first done.
-    by iExists _.
+    iFrame. by iExists _.
   Qed.
 
   Lemma sem_typed_nat_binop_bool P Γ op e1 e2 :
     binop_arithmetic_to_bool op = true →
-    P ; Γ ⊨ e1 : TNat -∗ P ; Γ ⊨ e2 : TNat -∗ P ; Γ ⊨ BinOp op e1 e2 : TBool.
+    P ;; Γ ⊨ e1 : TNat -∗ P ;; Γ ⊨ e2 : TNat -∗ P ;; Γ ⊨ BinOp op e1 e2 : TBool.
   Proof.
     iIntros (Hop) "#IH1 #IH2". iIntros (Δ vs) "!# #HΓ #HP /=".
-    iApply (interp_expr_bind [BinOpRCtx _ _]); first by iApply "IH2".
+    iApply (interp_expr_bind [BinOpRCtx _ _]); first (by iApply "IH2"; last done).
     iIntros (v) "#Hv /=".
-    iApply (interp_expr_bind [BinOpLCtx _ _]); first by iApply "IH1".
-    iIntros (w) "#Hw/=".
+    iApply (interp_expr_bind [BinOpLCtx _ _]); first (by iApply "IH1"; last done).
+    iIntros (w) "#Hw/= Htok".
     iDestruct "Hv" as (n) "%"; iDestruct "Hw" as (n') "%"; simplify_eq/=.
     assert (exists (r:bool), bin_op_eval op (#n') (#n) = Some (#r)) as [b Hb].
     1: { destruct op. 1-10,13: cbn in Hop; done.
          all: unfold bin_op_eval; destruct decide; simplify_eq.
          all: cbn; destruct bool_decide; by eexists. }
     iApply wp_pure_step_later; [done|]; iIntros "!>". iApply wp_value; first done.
-    by iExists _.
+    iFrame. by iExists _.
   Qed.
 
   Lemma sem_typed_bool_binop P Γ op e1 e2 :
     binop_boolish op = true →
-    P ; Γ ⊨ e1 : TBool -∗ P ; Γ ⊨ e2 : TBool -∗ P ; Γ ⊨ BinOp op e1 e2 : TBool.
+    P ;; Γ ⊨ e1 : TBool -∗ P ;; Γ ⊨ e2 : TBool -∗ P ;; Γ ⊨ BinOp op e1 e2 : TBool.
   Proof.
     iIntros (Hop) "#IH1 #IH2". iIntros (Δ vs) "!# #HΓ #HP /=".
-    iApply (interp_expr_bind [BinOpRCtx _ _]); first by iApply "IH2".
+    iApply (interp_expr_bind [BinOpRCtx _ _]); first (by iApply "IH2"; last done).
     iIntros (v) "#Hv /=".
-    iApply (interp_expr_bind [BinOpLCtx _ _]); first by iApply "IH1".
-    iIntros (w) "#Hw/=".
+    iApply (interp_expr_bind [BinOpLCtx _ _]); first (by iApply "IH1"; last done).
+    iIntros (w) "#Hw/= Htok".
     iDestruct "Hv" as (b) "%"; iDestruct "Hw" as (b') "%"; simplify_eq/=.
     assert (exists (r:bool), bin_op_eval op (#b') (#b) = Some (#r)) as [br Hbr].
     1: { destruct op. all: cbn in Hop; try done.
          all: unfold bin_op_eval; destruct decide; simplify_eq.
          all: by eexists. }
     iApply wp_pure_step_later; [done|]; iIntros "!>". iApply wp_value; first done.
-    by iExists _.
+    iFrame. by iExists _.
   Qed.
 
   Lemma sem_typed_eq P Γ τ e1 e2 :
     EqType τ →
-    P ; Γ ⊨ e1 : τ -∗ P ; Γ ⊨ e2 : τ -∗ P ; Γ ⊨ BinOp EqOp e1 e2 : TBool.
+    P ;; Γ ⊨ e1 : τ -∗ P ;; Γ ⊨ e2 : τ -∗ P ;; Γ ⊨ BinOp EqOp e1 e2 : TBool.
   Proof.
     iIntros (Hop) "#IH1 #IH2". iIntros (Δ vs) "!# #HΓ #HP /=".
-    iApply (interp_expr_bind [BinOpRCtx _ _]); first by iApply "IH2".
+    iApply (interp_expr_bind [BinOpRCtx _ _]); first (by iApply "IH2"; last done).
     iIntros (v) "#Hv /=".
-    iApply (interp_expr_bind [BinOpLCtx _ _]); first by iApply "IH1".
-    iIntros (w) "#Hw/=". inversion Hop. all: cbn.
+    iApply (interp_expr_bind [BinOpLCtx _ _]); first (by iApply "IH1"; last done).
+    iIntros (w) "#Hw/= Htok". inversion Hop. all: cbn.
     1: iDestruct "Hv" as "%"; iDestruct "Hw" as "%"; simplify_eq/=.
     2,3: iDestruct "Hv" as (v1) "%"; iDestruct "Hw" as (v2) "%"; simplify_eq/=.
     4: iDestruct "Hv" as (v1) "[% #H1]"; iDestruct "Hw" as (v2) "[% #H2]"; simplify_eq/=.
     all: iApply wp_pure_step_later; first by eauto.
     all: iIntros "!>"; iApply wp_value; first done.
-    all: by iExists _.
+    all: iFrame; by iExists _.
   Qed.
 
-  Lemma sem_typed_pair P Γ e1 e2 τ1 τ2 : P ; Γ ⊨ e1 : τ1 -∗ P ; Γ ⊨ e2 : τ2 -∗ P ; Γ ⊨ Pair e1 e2 : TProd τ1 τ2.
+  Lemma sem_typed_pair P Γ e1 e2 τ1 τ2 : P ;; Γ ⊨ e1 : τ1 -∗ P ;; Γ ⊨ e2 : τ2 -∗ P ;; Γ ⊨ Pair e1 e2 : TProd τ1 τ2.
   Proof.
     iIntros "#IH1 #IH2" (Δ vs) "!# #HΓ #HP"; simpl.
     iApply (interp_expr_bind [PairRCtx _]); first by iApply "IH2".
     iIntros (v) "#Hv /=".
     iApply (interp_expr_bind [PairLCtx _]); first by iApply "IH1".
-    iIntros (w) "#Hw/=".
+    iIntros (w) "#Hw/= Htok".
     iApply wp_pure_step_later; first done. iIntros "!>".
-    iApply wp_value; simpl; eauto.
+    iApply wp_value; simpl; eauto; iFrame; eauto.
   Qed.
 
-  Lemma sem_typed_fst P Γ e τ1 τ2 : P ; Γ ⊨ e : TProd τ1 τ2 -∗ P ; Γ ⊨ Fst e : τ1.
+  Lemma sem_typed_fst P Γ e τ1 τ2 : P ;; Γ ⊨ e : TProd τ1 τ2 -∗ P ;; Γ ⊨ Fst e : τ1.
   Proof.
     iIntros "#IH" (Δ vs) "!# #HΓ #HP"; simpl.
     iApply (interp_expr_bind [FstCtx]); first by iApply "IH".
     iIntros (v) "#Hv /=".
     iDestruct "Hv" as (w1 w2) "#[% [H2 H3]]"; subst.
-    iApply wp_pure_step_later; [done|]; iIntros "!>". by iApply wp_value.
+    iIntros "Htok".
+    iApply wp_pure_step_later; [done|]; iIntros "!>". iApply wp_value; eauto.
   Qed.
 
-  Lemma sem_typed_snd P Γ e τ1 τ2 : P ; Γ ⊨ e : TProd τ1 τ2 -∗ P ; Γ ⊨ Snd e : τ2.
+  Lemma sem_typed_snd P Γ e τ1 τ2 : P ;; Γ ⊨ e : TProd τ1 τ2 -∗ P ;; Γ ⊨ Snd e : τ2.
   Proof.
     iIntros "#IH" (Δ vs) "!# #HΓ #HP"; simpl.
     iApply (interp_expr_bind [SndCtx]); first by iApply "IH".
     iIntros (v) "#Hv /=".
     iDestruct "Hv" as (w1 w2) "#[% [H2 H3]]"; subst.
-    iApply wp_pure_step_later; [done|]; iIntros "!>". by iApply wp_value.
+    iIntros "Htok".
+    iApply wp_pure_step_later; [done|]; iIntros "!>". iApply wp_value; eauto.
   Qed.
 
-  Lemma sem_typed_injl P Γ e τ1 τ2 : P ; Γ ⊨ e : τ1 -∗ P ; Γ ⊨ InjL e : (TSum τ1 τ2).
+  Lemma sem_typed_injl P Γ e τ1 τ2 : P ;; Γ ⊨ e : τ1 -∗ P ;; Γ ⊨ InjL e : (TSum τ1 τ2).
   Proof.
     iIntros "#IH" (Δ vs) "!# #HΓ #HP"; simpl.
     iApply (interp_expr_bind [InjLCtx]); first by iApply "IH".
     iIntros (v) "#Hv /=".
+    iIntros "Htok".
     iApply wp_pure_step_later; first done. iIntros "!>".
     iApply wp_value; simpl; eauto.
   Qed.
 
-  Lemma sem_typed_injr P Γ e τ1 τ2 : P ; Γ ⊨ e : τ2 -∗ P ; Γ ⊨ InjR e : TSum τ1 τ2.
+  Lemma sem_typed_injr P Γ e τ1 τ2 : P ;; Γ ⊨ e : τ2 -∗ P ;; Γ ⊨ InjR e : TSum τ1 τ2.
   Proof.
     iIntros "#IH" (Δ vs) "!# #HΓ #HP"; simpl.
     iApply (interp_expr_bind [InjRCtx]); first by iApply "IH".
     iIntros (v) "#Hv /=".
+    iIntros "Htok".
     iApply wp_pure_step_later; first done. iIntros "!>".
     iApply wp_value; simpl; eauto.
   Qed.
 
   Lemma sem_typed_case P Γ e0 e1 e2 τ1 τ2 τ3 :
-    P ; Γ ⊨ e0: TSum τ1 τ2 -∗
-    P ; Γ ⊨ e1 : (TArrow τ1 τ3) -∗
-    P ; Γ ⊨ e2 : (TArrow τ2 τ3) -∗
-    P ; Γ ⊨ Case e0 e1 e2 : τ3.
+    P ;; Γ ⊨ e0: TSum τ1 τ2 -∗
+    P ;; Γ ⊨ e1 : (TArrow τ1 τ3) -∗
+    P ;; Γ ⊨ e2 : (TArrow τ2 τ3) -∗
+    P ;; Γ ⊨ Case e0 e1 e2 : τ3.
   Proof.
     iIntros "#IH1 #IH2 #IH3" (Δ vs) "!# #HΓ #HP"; simpl.
     iApply (interp_expr_bind [CaseCtx _ _]); first by iApply "IH1".
     iIntros (v) "#Hv /=".
     iDestruct "Hv" as "[Hv|Hv]"; iDestruct "Hv" as (w) "[% Hw]"; simplify_eq/=.
-    + iApply wp_pure_step_later; auto 1 using to_of_val; asimpl. iIntros "!>".
+    + iIntros "Htok".
+      iApply wp_pure_step_later; auto 1 using to_of_val; asimpl. iIntros "!>".
       iPoseProof ("IH2" $! Δ vs with "HΓ HP") as "IH".
-      iApply (interp_expr_bind [AppLCtx _]); first by iApply "IH".
+      iApply (interp_expr_bind [AppLCtx _]); first (by iApply "IH"); last iFrame.
       iIntros (v) "#Hv". by iApply "Hv".
-    + iApply wp_pure_step_later; auto 1 using to_of_val; asimpl. iIntros "!>".
+    + iIntros "Htok".
+      iApply wp_pure_step_later; auto 1 using to_of_val; asimpl. iIntros "!>".
       iPoseProof ("IH3" $! Δ vs with "HΓ HP") as "IH".
-      iApply (interp_expr_bind [AppLCtx _]); first by iApply "IH".
+      iApply (interp_expr_bind [AppLCtx _]); first (by iApply "IH"); last iFrame.
       iIntros (v) "#Hv". by iApply "Hv".
   Qed.
 
   Lemma sem_typed_if P Γ e0 e1 e2 τ :
-    P ; Γ ⊨ e0 : TBool -∗ P ; Γ ⊨ e1 : τ -∗ P ; Γ ⊨ e2 : τ -∗ P ; Γ ⊨ If e0 e1 e2 : τ.
+    P ;; Γ ⊨ e0 : TBool -∗ P ;; Γ ⊨ e1 : τ -∗ P ;; Γ ⊨ e2 : τ -∗ P ;; Γ ⊨ If e0 e1 e2 : τ.
   Proof.
     iIntros "#IH1 #IH2 #IH3" (Δ vs) "!# #HΓ #HP"; simpl.
     iApply (interp_expr_bind [IfCtx _ _]); first by iApply "IH1".
-    iIntros (v) "(%&->) /=". destruct b;
+    iIntros (v) "(%&->) /= Htok". destruct b;
     (iApply wp_pure_step_later; first done); iIntros "!>";
       [iApply "IH2"| iApply "IH3"]; auto.
   Qed.
@@ -198,20 +209,20 @@ Section typed_interp.
   Qed.
 
   Lemma sem_typed_rec P Γ f x e τ1 τ2 :
-    P ; (binder_insert f (TArrow τ1 τ2) (binder_insert x τ1 Γ)) ⊨ e : τ2 -∗ P ; Γ ⊨ Rec f x e : TArrow τ1 τ2.
+    P ;; (binder_insert f (TArrow τ1 τ2) (binder_insert x τ1 Γ)) ⊨ e : τ2 -∗ P ;; Γ ⊨ Rec f x e : TArrow τ1 τ2.
   Proof.
-    iIntros "#IH" (Δ vs) "!# #HΓ #HP"; simpl.
+    iIntros "#IH" (Δ vs) "!# #HΓ #HP Htok"; simpl.
     iApply wp_pure_step_later; first done; iIntros "!>".
-    iApply wp_value; first done. iLöb as "IHL". cbn.
-    iIntros "!> %v #Hv".
+    iApply wp_value; first done. iFrame "Htok". iLöb as "IHL". cbn.
+    iIntros "!> %v #Hv Htok".
     iApply wp_pure_step_later; first done; iIntros "!>".
     rewrite (binder_delete_binder_delete f x) /env_subst -(subst_all_binder_insert_2).
-    iApply ("IH" $! Δ with "[HΓ] HP").
+    iApply ("IH" $! Δ with "[HΓ] HP"); last done.
     iApply (interp_env_binder_insert_2 with "[IHL] [-]"); first iApply "IHL".
     iApply (interp_env_binder_insert_2 with "Hv HΓ").
   Qed.
 
-  Lemma sem_typed_app P Γ e1 e2 τ1 τ2 : P ; Γ ⊨ e1 : TArrow τ1 τ2 -∗ P ; Γ ⊨ e2 : τ1 -∗ P ; Γ ⊨ App e1 e2 :  τ2.
+  Lemma sem_typed_app P Γ e1 e2 τ1 τ2 : P ;; Γ ⊨ e1 : TArrow τ1 τ2 -∗ P ;; Γ ⊨ e2 : τ1 -∗ P ;; Γ ⊨ App e1 e2 :  τ2.
   Proof.
     iIntros "#IH1 #IH2" (Δ vs) "!# #HΓ #HP"; simpl.
     iApply (interp_expr_bind [AppRCtx _]); first by iApply "IH2".
@@ -221,128 +232,160 @@ Section typed_interp.
     iApply "Hw"; done.
   Qed.
 
-  Lemma sem_typed_tlam P Γ e τ : subst_prog_env (ren (+1)) P ; (subst (ren (+1)) <$> Γ) ⊨ e : τ -∗ P ; Γ ⊨ TLam e : TForall τ.
+  Lemma sem_typed_tlam P Γ e τ : subst_prog_env (ren (+1)) P ;; (subst (ren (+1)) <$> Γ) ⊨ e : τ -∗ P ;; Γ ⊨ TLam e : TForall τ.
   Proof.
-    iIntros "#IH" (Δ vs) "!# #HΓ #HP /=".
+    iIntros "#IH" (Δ vs) "!# #HΓ #HP /= Htok".
     iApply wp_pure_step_later; first done; iIntros "!>".
-    iApply wp_value; first done. cbn.
-    iModIntro; iIntros (τi).
+    iApply wp_value; first done. cbn. iFrame "Htok".
+    iModIntro; iIntros (τi) "Htok".
     iApply wp_pure_step_later; first done. iIntros "!>". cbn.
-    iApply "IH". 1: by iApply interp_env_ren.
+    iApply "IH"; last done. 1: by iApply interp_env_ren.
     by iApply interp_prog_env_ren.
   Qed.
 
-  Lemma sem_typed_tapp P Γ e τ τ' : P ; Γ ⊨ e : TForall τ -∗ P ; Γ ⊨ TApp e : τ.[τ'/].
+  Lemma sem_typed_tapp P Γ e τ τ' : P ;; Γ ⊨ e : TForall τ -∗ P ;; Γ ⊨ TApp e : τ.[τ'/].
   Proof.
     iIntros "#IH" (Δ vs) "!# #HΓ #HP /=".
     iApply (interp_expr_bind [AppLCtx _]); first by iApply "IH". cbn.
-    iIntros (v) "#Hv /=".
+    iIntros (v) "#Hv /= Htok".
     iApply wp_wand_r; iSplitL;
-      [iApply ("Hv" $! (⟦ τ' ⟧ Δ)); iPureIntro; apply _|]; cbn.
-    iIntros (w) "?". by iApply interp_subst.
+      [iApply ("Hv" $! (⟦ τ' ⟧ Δ)); last done; iPureIntro; apply _|]; cbn.
+    iIntros (w) "[? $]". by iApply interp_subst.
   Qed.
 
-  Lemma sem_typed_pack P Γ e τ τ' : P ; Γ ⊨ e : τ.[τ'/] -∗ P ; Γ ⊨ Pack e : TExist τ.
+  Lemma sem_typed_pack P Γ e τ τ' : P ;; Γ ⊨ e : τ.[τ'/] -∗ P ;; Γ ⊨ Pack e : TExist τ.
   Proof.
-    iIntros "#IH" (Δ vs) "!# #HΓ #HP /=".
-    iApply wp_wand; first by iApply "IH".
-    iIntros (v) "#Hv /=".
+    iIntros "#IH" (Δ vs) "!# #HΓ #HP /= Htok".
+    iApply (wp_wand with "[Htok]"); first by iApply "IH".
+    iIntros (v) "[#Hv $] /=".
     rewrite -interp_subst.
     iExists (interp _ _ Δ), _; iSplit; done.
   Qed.
 
   Lemma sem_typed_unpack P Γ x e1 e2 τ τ' :
-    P ; Γ ⊨ e1 : TExist τ -∗
-    subst_prog_env (ren (+1)) P ; binder_insert x τ (subst (ren (+1)) <$> Γ) ⊨ e2 : τ'.[ren (+1)]  -∗
-    P ; Γ ⊨ UnpackIn x e1 e2 : τ'.
+    P ;; Γ ⊨ e1 : TExist τ -∗
+    subst_prog_env (ren (+1)) P ;; binder_insert x τ (subst (ren (+1)) <$> Γ) ⊨ e2 : τ'.[ren (+1)]  -∗
+    P ;; Γ ⊨ UnpackIn x e1 e2 : τ'.
   Proof.
     iIntros "#IH1 #IH2" (Δ vs) "!# #HΓ #HP /=".
     iApply (interp_expr_bind [AppRCtx _]); first by iApply "IH1". cbn.
-    iIntros (v) "#(%τi & %vv & -> & Hv) /=".
+    iIntros (v) "#(%τi & %vv & -> & Hv) /= Htok".
     iApply (wp_bind [AppLCtx _]); first iApply (wp_wand _ _ _ (λ v, ⌜v = (λ: x, env_subst (delete_binder vs x) e2)%MLV⌝)%I).
     1: iApply wp_pure_step_later; first done; iIntros "!>". 1: iApply wp_value; first done; iPureIntro; done.
     iIntros (?) "->". cbn.
     iApply wp_pure_step_later; first done. iIntros "!>". cbn.
     rewrite -subst_all_binder_insert.
     iApply wp_wand_r; iSplitL.
-    { iApply ("IH2" $! (τi :: Δ) with "[]").
+    { iApply ("IH2" $! (τi :: Δ) with "[]"); last done.
       1: iApply interp_env_binder_insert_2; first iApply "Hv".
       1: iApply interp_env_ren; done.
       1: iApply interp_prog_env_ren; done. }
-    iIntros (u) "Hu".
+    iIntros (u) "[Hu $]".
     iApply (interp_weaken _ [] [_]); done.
   Qed.
 
-  Lemma sem_typed_fold P Γ e τ : P ; Γ ⊨ e : τ.[(TRec τ)/] -∗ P ; Γ ⊨ Roll e : TRec τ.
+  Lemma sem_typed_fold P Γ e τ : P ;; Γ ⊨ e : τ.[(TRec τ)/] -∗ P ;; Γ ⊨ Roll e : TRec τ.
   Proof.
     iIntros "#IH" (Δ vs) "!# #HΓ #HP /=".
     iApply (interp_expr_bind [AppRCtx _]); first by iApply "IH".
-    iIntros (v) "#Hv /=".
+    iIntros (v) "#Hv /= Htok".
     iApply wp_pure_step_later; first done; iIntros "!>"; cbn.
     rewrite lookup_singleton.
     iApply wp_value; first done.
     rewrite /= -interp_subst fixpoint_interp_rec1_eq /=.
-    iModIntro; eauto.
+    iFrame. iModIntro; eauto.
   Qed.
 
-  Lemma sem_typed_unfold P Γ e τ : P ; Γ ⊨ e : TRec τ -∗ P ; Γ ⊨ Unroll e : τ.[(TRec τ)/].
+  Lemma sem_typed_unfold P Γ e τ : P ;; Γ ⊨ e : TRec τ -∗ P ;; Γ ⊨ Unroll e : τ.[(TRec τ)/].
   Proof.
     iIntros "#IH" (Δ vs) "!# #HΓ #HP /=".
     iApply (interp_expr_bind [AppRCtx _]); first by iApply "IH".
     iIntros (v) "#Hv /=".
     rewrite /= fixpoint_interp_rec1_eq.
     change (fixpoint _) with (⟦ TRec τ ⟧ Δ); simpl.
-    iDestruct "Hv" as (w) "#[% Hw]"; subst.
+    iDestruct "Hv" as (w) "#[% Hw]"; subst. iIntros "Htok".
     iApply wp_pure_step_later; cbn; auto using to_of_val. rewrite lookup_singleton.
-    iIntros "!>". iApply wp_value; first done. by iApply interp_subst.
+    iIntros "!>". iApply wp_value; first done. iFrame. by iApply interp_subst.
   Qed.
 
-  Lemma sem_typed_alloc P Γ e τ : P ; Γ ⊨ e : τ -∗ P ; Γ ⊨ Alloc e : Tref τ.
-  Proof.
-    iIntros "#IH" (Δ vs) "!# #HΓ #HP /=".
-    iApply (interp_expr_bind [AllocNRCtx _]); first by iApply "IH".
-    iIntros (v) "#Hv /=". unfold interp_expr.
-    wp_alloc l as "Hl".
-    iMod (inv_alloc _ with "[Hl]") as "#HN".
-    2: iModIntro; cbn; iExists l; by iSplit.
-    iNext; iExists _; by iFrame.
-  Qed.
-
-(* TODO: figure out invariants
-
-  Lemma sem_typed_load P Γ e τ : P ; Γ ⊨ e : (Tref τ) -∗ P ; Γ ⊨ Load e : τ.
-  Proof.
-    iIntros "#IH" (Δ vs) "!# #HΓ #HP /=".
-    iApply (interp_expr_bind [LoadNLCtx _]); first by iApply "IH".
-    rewrite /= /fill /=.
-    iIntros (v) "#(%l&->&#Hv) /=".
-    Search inv.
-    iApply wp_atomic.
-    iInv (logN .@ l) as (w) "[Hw1 #Hw2]" "Hclose".
-    iApply (wp_load with "Hw1").
-    iModIntro. iNext.
-    iIntros "Hw1". iMod ("Hclose" with "[Hw1 Hw2]"); eauto.
-  Qed.
-
-  Lemma sem_typed_store Γ e1 e2 τ : P ; Γ ⊨ e1 : (Tref τ) -∗ P ; Γ ⊨ e2 : τ -∗ P ; Γ ⊨ Store e1 e2 : TUnit.
+  Lemma sem_typed_alloc P Γ e1 e2 τ :
+    P ;; Γ ⊨ e1 : TNat -∗
+    P ;; Γ ⊨ e2 : τ -∗
+    P ;; Γ ⊨ AllocN e1 e2 : TArray τ.
   Proof.
     iIntros "#IH1 #IH2" (Δ vs) "!# #HΓ #HP /=".
-    iApply (interp_expr_bind [StoreLCtx _]); first by iApply "IH1".
-    iIntros (v) "#Hv /=".
-    iApply (interp_expr_bind [StoreRCtx _]); first by iApply "IH2".
-    iIntros (w) "#Hw/=".
-    iDestruct "Hv" as (l) "[% #Hv]"; subst.
-    iApply wp_atomic.
-    iInv (logN .@ l) as (z) "[Hz1 #Hz2]" "Hclose".
-    iApply (wp_store with "Hz1"); auto using to_of_val.
-    iModIntro. iNext.
-    iIntros "Hz1". iMod ("Hclose" with "[Hz1 Hz2]"); eauto.
-  Qed. *)
+    iApply (interp_expr_bind [AllocNRCtx _]); first by iApply "IH2".
+    iIntros (v2) "#Hv2 /=".
+    iApply (interp_expr_bind [AllocNLCtx _]); first by iApply "IH1".
+    iIntros (v1) "#(%n&->) /= Htok".
+    destruct (decide (0 ≤ n)%Z) as [Hn|Hn].
+    { wp_alloc l as "Hl"; first done. iFrame "Htok".
+      iMod (na_inv_alloc _ with "[Hl]") as "#HN".
+      2: { iModIntro. cbn. iExists l. by iSplit. }
+      iNext. iExists _. iFrame "Hl".
+      iApply big_sepL_forall. by iIntros (? ? (-> & _)%lookup_replicate). }
+    { iApply (wp_allocN_wrong_size with "[] []"); [lia|done|].
+      iIntros "!> ?". done. }
+  Qed.
+
+  Lemma sem_typed_load P Γ e1 e2 τ :
+    P ;; Γ ⊨ e1 : (TArray τ) -∗
+    P ;; Γ ⊨ e2 : TNat -∗
+    P ;; Γ ⊨ LoadN e1 e2 : τ.
+  Proof.
+    iIntros "#IH1 #IH2" (Δ vs) "!# #HΓ #HP /=".
+    iApply (interp_expr_bind [LoadNRCtx _]); first by iApply "IH2".
+    iIntros (v2) "#(%n2&->) /=".
+    iApply (interp_expr_bind [LoadNLCtx _]); first by iApply "IH1".
+    iIntros (v1) "#(%l&->&#Hv1) /= Htok"; rewrite -/(interp _).
+    iMod (na_inv_acc with "Hv1 Htok") as "[Hvs (Htok & Hclose)]"; [done..|].
+    iDestruct "Hvs" as (vv) "[Hvv #Hvvτ]".
+    destruct (decide (0 ≤ n2 < length vv)%Z) as [Hn2|Hn2].
+    { assert (is_Some (vv !! Z.to_nat n2)) as [v ?].
+      { apply lookup_lt_is_Some_2. lia. }
+      iApply wp_fupd.
+      iApply (wp_loadN with "Hvv"); [lia|eauto|].
+      iIntros "!> Hvv".
+      iMod ("Hclose" with "[Hvv Hvvτ $Htok]") as "$".
+      { iNext. iExists _. iFrame "Hvvτ ∗". }
+      iModIntro. by iApply (big_sepL_lookup with "Hvvτ"). }
+    { iApply (wp_loadN_oob with "Hvv"); first lia. by iIntros "!>" (?) "?". }
+  Qed.
+
+  Lemma sem_typed_store P Γ e1 e2 e3 τ :
+    P ;; Γ ⊨ e1 : (TArray τ) -∗
+    P ;; Γ ⊨ e2 : TNat -∗
+    P ;; Γ ⊨ e3 : τ -∗
+    P ;; Γ ⊨ StoreN e1 e2 e3 : TUnit.
+  Proof.
+    iIntros "#IH1 #IH2 #IH3" (Δ vs) "!# #HΓ #HP /=".
+    iApply (interp_expr_bind [StoreNRRCtx _ _]); first by iApply "IH3".
+    iIntros (v3) "#Hv3 /=".
+    iApply (interp_expr_bind [StoreNLRCtx _ _]); first by iApply "IH2".
+    iIntros (v2) "#(%n2&->)/=".
+    iApply (interp_expr_bind [StoreNLLCtx _ _]); first by iApply "IH1".
+    iIntros (v1) "#(%l&->&Hinv)/="; rewrite -/(interp _).
+    iIntros "Htok".
+    iMod (na_inv_acc with "Hinv Htok") as "[Hvs (Htok & Hclose)]"; [done..|].
+    iDestruct "Hvs" as (vv) "[Hvv #Hvvτ]".
+    destruct (decide (0 ≤ n2 < length vv)%Z) as [Hn2|Hn2].
+    { assert (is_Some (vv !! Z.to_nat n2)) as [v ?].
+      { apply lookup_lt_is_Some_2. lia. }
+      iApply wp_fupd.
+      iApply (wp_storeN with "Hvv"); first lia.
+      iIntros "!> Hvv".
+      iMod ("Hclose" with "[Hvv Hvvτ $Htok]") as "$".
+      { iNext. iExists _. iFrame "Hvv".
+        iDestruct (big_sepL_insert_acc with "Hvvτ") as "[_ H]"; first done.
+        by iApply "H". }
+      done. }
+    { iApply (wp_storeN_oob with "Hvv"); first lia. by iIntros "!>" (?) "?". }
+  Qed.
 
   Lemma sem_typed_extern_ind P Γ Δ vs s tr tl1 tl2 vl1 el2 :
       P !! s = Some (FunType (tl1 ++ tl2) tr) →
       ⟦ Γ ⟧* Δ vs -∗ ⟦ P ⟧ₚ* Δ -∗
-      ⌜Forall2 (λ e τ, ⊢ P; Γ ⊨ e : τ) el2 tl2⌝ -∗
+      ⌜Forall2 (λ e τ, ⊢ P ;; Γ ⊨ e : τ) el2 tl2⌝ -∗
       ([∗ list] k↦τ;v ∈ tl1;vl1, ⟦ τ ⟧ Δ v) -∗
       (⟦ tr ⟧ₑ Δ) (Extern s (map Val vl1 ++ map (env_subst vs) el2)).
   Proof.
@@ -369,14 +412,14 @@ Section typed_interp.
 
   Lemma sem_typed_extern P Γ s el tl tr :
       P !! s = Some (FunType tl tr) →
-      ⌜Forall2 (λ e τ, ⊢ P ; Γ ⊨ e : τ) el tl⌝ -∗
-      P ; Γ ⊨ (Extern s el) : tr.
+      ⌜Forall2 (λ e τ, ⊢ P ;; Γ ⊨ e : τ) el tl⌝ -∗
+      P ;; Γ ⊨ (Extern s el) : tr.
   Proof.
     iIntros (Hlu HH Δ vs) "!# #HΓ #HP /=".
     by iApply (sem_typed_extern_ind P Γ Δ vs s tr [] tl [] el).
   Qed.
 
-  Theorem fundamental P Γ e τ : typed P Γ e τ → ⊢ P ; Γ ⊨ e : τ.
+  Theorem fundamental P Γ e τ : typed P Γ e τ → ⊢ P ;; Γ ⊨ e : τ.
   Proof.
     induction 1.
     - iApply sem_typed_var; done.
@@ -403,8 +446,8 @@ Section typed_interp.
     - iApply sem_typed_fold; done.
     - iApply sem_typed_unfold; done.
     - iApply sem_typed_alloc; done.
-    - admit.
-    - admit.
+    - iApply sem_typed_load; done.
+    - iApply sem_typed_store; done.
     - iApply sem_typed_extern; done.
-  Admitted.
+  Qed.
 End typed_interp.
